Proved progress and most of preservation using Nik's suggestion
Still have to figure out how to instantiate the substitution lemma.
And still have to prove the substitution lemma, and a couple other ones.

examples/unit-tests/stlc.fst
@@ -92,7 +92,7 @@ let extend_eq g x a = ()
 
 val extend_neq : g:env -> x1:int -> a:ty -> x2:int -> Pure unit
       (requires (x2 =!= x1))
-      (ensures \r => ((extend g x2 a) x1) = g x1)
+      (ensures \r -> ((extend g x2 a) x1) = g x1)
 let extend_neq g x1 a x2 = ()
 
 (* CH: swapped env and exp args until functions are ignored from the
@@ -122,17 +122,27 @@ let rec typing e g =
 
 val canonical_forms_bool : e:exp -> Pure unit
       (requires ((typing e empty = Some TBool) /\ (is_value e = true)))
-      (ensures \r => (e = ETrue) \/ (e = EFalse))
+      (ensures \r -> (e = ETrue) \/ (e = EFalse))
 let canonical_forms_bool e =
   match e with
   | EVar x -> ()
-  | EAbs x' t e1 ->
-      (* strange that F* can't prove this simple case *)
-      (* This fails now, but maybe if we manage to get rid of the existentials
-         by replacing them with testers and projectors?
-      assert(exists (t1:ty). exists (t2:ty).
-               typing (EAbs x' t e1) = Some (TArrow t1 t2)); *)
+  | EAbs x' t e1 -> begin
       admit()
+      (* that F* can't prove this simple case, we should get a contradition *)
+      (* This assert fails
+      assert(exists (t1:ty). exists (t2:ty).
+               typing (EAbs x' t e1) empty = Some (TArrow t1 t2) \/
+               typing (EAbs x' t e1) empty = None);  *)
+     (* this causes the whole thing to explode! 3 different bogus errors
+      match typing e1 (extend empty x' t) with
+      | Some t' -> admit()
+      | None    -> admit() *)
+      (* this doesn't bring much
+      match typing e empty with
+      | Some (TArrow t1 t2) -> ()
+      | Some TBool -> admit()
+      | _ -> () *)
+      end
   | EApp e1 e2 -> ()
   | ETrue -> ()
   | EFalse -> ()
@@ -140,33 +150,45 @@ let canonical_forms_bool e =
 
 val canonical_forms_fun : e:exp -> t1:ty -> t2:ty -> Pure unit
       (requires ((typing e empty = Some (TArrow t1 t2)) /\ (is_value e = true)))
-      (ensures \r => (is_EAbs e))
+      (ensures \r -> (is_EAbs e))
 let canonical_forms_fun e t1 t2 = ()
+
+(* "An unknown assertion in the term at this location was not provable."
+   No wonder that the first case of progress fails.
+   Logic encoding of empty looks reasonable, Z3 should be able to prove this.
+   Is the encoding of is_None broken? I wasn't able to find any equations for it.
+   Only Prims.fst and Prims.snd get equations? Really? *)
+val sel_empty : x:int -> Fact unit
+      (ensures (is_None (empty x)))
+let sel_empty x = ()
+
+(* "An unknown assertion in the term at this location was not provable."
+   The (for some reason) unprovable query looks like this:
+   (= (Prims.op_Equality (Prims.option Stlc.ty)
+                         (Stlc.empty x___844)
+                         (Prims.None Stlc.ty))
+      (BoxBool true))
+*)
+
+val sel_empty' : x:int -> Fact unit
+      (ensures (empty x = None))
+let sel_empty' x = ()
 
 val progress : e:exp -> t:ty -> Pure unit
       (requires (typing e empty = Some t))
-      (ensures \r => (is_value e \/ (is_Some (step e))))
+      (ensures \r -> (is_value e \/ (is_Some (step e))))
 let rec progress e t =
   match e with
   | EVar x ->
-      (* assert(typing (EVar x) empty = None); -- this fails *)
+      (* assert(typing (EVar x) empty = None);
+         -- this fails and it shouldn't; the case should be trivial *)
       admit()
   | EAbs x' t e1 -> ()
-  | EApp e1 e2 ->
-(* problem: for progress e1 and progress e2 we don't have anything to
-   pass for t; implicit lemma instantiation might help for such cases *)
-      assert(exists (t1:ty). exists (t2:ty).
-               typing e1 empty = Some (TArrow t1 t2) /\
-               typing e2 empty = Some t1);
-          (* The assert is proved, but it's not enough.
-             We want to apply progress for the existentially
-             quantified t1 and t2 above! How can we do that?
-             If we prove unique existence for something logical
-             can we somehow soundly expose it back to F*? *)
-      if is_value e1 then
-        if is_value e2 then ()
-        else admit()
-      else admit()
+  | EApp e1 e2 -> begin
+      match typing e1 empty with
+      | Some (TArrow t1 t2) ->
+          progress e1 (TArrow t1 t2); progress e2 t1
+      end
   | ETrue -> ()
   | EFalse -> ()
   | EIf e1 e2 e3 ->
@@ -187,27 +209,62 @@ type closed e = (forall (x:int). not (appears_free_in x e))
 
 val free_in_context : x:int -> e:exp -> t:ty -> g:env -> Pure unit
       (requires (appears_free_in x e = true /\ typing e g = Some t))
-      (ensures \r => (is_Some (g x)))
+      (ensures \r -> (is_Some (g x)))
 let free_in_context x e t g = ()
 
 val context_invariance : g:env -> g':env -> e:exp -> t:ty -> Pure unit
       (requires (typing e g = Some t /\
                    (forall (x:int). appears_free_in x e = true ==>
                                     g x = g' x)))
-      (ensures \r => (typing e g' = Some t))
+      (ensures \r -> (typing e g' = Some t))
 let context_invariance g g' e t = ()
 
 val substitution_preserves_typing :
       g:env -> x:int -> e:exp -> u:ty -> t:ty -> v:exp -> Pure unit
           (requires (typing e (extend g x u) = Some t /\
                        (typing v empty = Some u)))
-          (ensures \r => (typing (subst x v e) g = Some t))
+          (ensures \r -> (typing (subst x v e) g = Some t))
 let substitution_preserves_typing g x e u t v = ()
 
 val preservation : e:exp -> e':exp -> t:ty -> Pure unit
       (requires (typing e empty = Some t /\ step e = Some e'))
-      (ensures \r => (typing e' empty = Some t))
-let preservation e e' t = ()
+      (ensures \r -> (typing e' empty = Some t))
+let rec preservation e e' t =
+  match e with
+  | EVar _ -> ()
+  | EAbs _ _ _ -> ()
+  | EApp e1 e2 -> begin
+      match typing e1 empty with
+      | Some (TArrow t1 t2) -> begin
+          assert(typing e2 empty = Some t1); (* -- works *)
+          assert(typing e empty = Some t2); (* -- works *)
+          if is_value e1 then
+            if is_value e2 then
+              match e1 with
+              | EAbs x t e' ->
+                  assert(step e = Some (subst x e2 e')); (* -- works *)
+(*                  assert (t = t1); -- this should work, but it doesn't *)
+(*                  assert(typing e' (extend empty x t1) = Some t2);
+                      -- this should work, but it doesn't *)
+(*                  substitution_preserves_typing empty x e' t1 t2 e2
+                      -- this should work, but now precondition fails *)
+                  admit()
+            else
+              match (step e2) with
+              | Some e2' -> preservation e2 e2' t1
+          else
+            match (step e1) with
+            | Some e1' -> preservation e1 e1' (TArrow t1 t2)
+          end
+      end
+  | ETrue -> ()
+  | EFalse -> ()
+  | EIf e1 _ _ ->
+      if is_value e1 then ()
+      else begin
+        match (step e1) with
+        | Some e1' -> preservation e1 e1' TBool
+      end
 
 (* CH: With this purely-executable way of specifying things we can't
    do rule induction, and that is restrictive and will probably lead
